src/study/Nemonuri.Study.CSharpSyntaxRewriter2.Modifier2/Nemonuri.StratifiedNodes.Nodes.Children.fst
@@ -1,0 +1,28 @@
+module Nemonuri.StratifiedNodes.Nodes.Children
+
+module L = FStar.List.Tot
+module Math = FStar.Math.Lib
+module I = Nemonuri.StratifiedNodes.Internals
+module T = Nemonuri.StratifiedNodes.Nodes.Base.Types
+open Nemonuri.StratifiedNodes.Nodes.Base.Members
+open Nemonuri.StratifiedNodes.Nodes.Bijections
+
+//--- theory members ---
+let get_children #t (node:T.node t) : Tot (T.node_list t) =
+  to_node_list node.internal.children
+
+let get_children_length #t (node:T.node  t) 
+  : Pure nat (requires True) (ensures fun r -> r = L.length (get_children node)) = 
+  I.get_length node.internal.children
+//---|
+
+//--- private theory members ---
+let get_child_at #t (nd:T.node  t) (index:nat)
+  : Pure (T.node  t) 
+    (requires (index < (get_children_length nd)))
+    (ensures fun r -> r = (L.index (get_children nd) index))
+  =
+  // TODO: Internals 단계에서 구현하기
+  L.index (get_children nd) index
+
+//---|
